fsub/autosubst2_dctx/prop_basic.v
@@ -1,0 +1,55 @@
+Require Import common.prop_as_core.
+Require Import common.prop_as_unscoped.
+Require Import fsub.autosubst2_dctx.def_as2.
+Require Import fsub.autosubst2_dctx.def_extra.
+
+From Coq Require Import ssreflect ssrfun ssrbool.
+From Hammer Require Import Tactics.
+Require Import Coq.Program.Equality.
+Require Import List.
+
+Import SubstNotations.
+Import UnscopedNotations.
+
+Definition ctx_tvar_rename_weak Δ Δ' ξ :=
+  forall X B, lookup_tvar X Δ B -> exists B', lookup_tvar (ξ X) Δ' B'.
+
+Definition ctx_tvar_rename Δ Δ' ξ :=
+  forall X B, lookup_tvar X Δ B -> lookup_tvar (ξ X) Δ' (B ⟨ ξ ⟩).
+
+Lemma wf_typ_weaken_tvar Δ Δ' A ξ:
+  Δ ⊢ A ->
+  ctx_tvar_rename_weak Δ Δ' ξ ->
+  Δ' ⊢ A ⟨ ξ ⟩.
+Proof.
+  move: Δ Δ' ξ. induction A; try hauto.
+  - intros. unfold ctx_tvar_rename_weak in *.
+    asimpl. simpl in *. 
+    hauto inv:lookup_tvar ctrs:lookup_tvar.
+Qed.
+
+Corollary wf_typ_weaken_tvar0 Δ A B:
+  Δ ⊢ A ->
+  (B :: Δ) ⊢ A ⟨↑⟩.
+Proof.
+  hauto unfold:ctx_tvar_rename_weak inv:lookup_tvar ctrs:lookup_tvar
+    use:wf_typ_weaken_tvar.
+Qed.
+
+Lemma sub_weaken_tvar  Δ Δ' A B ξ :
+  Δ ⊢ A <: B ->
+  ctx_tvar_rename Δ Δ' ξ ->
+  Δ' ⊢ A ⟨ ξ ⟩ <: B ⟨ ξ ⟩.
+Proof.
+  move => H.
+  move: Δ' ξ. elim: Δ A B / H; intros; 
+    try hauto unfold:ctx_tvar_rename,ctx_tvar_rename_weak ctrs:subtyping use:wf_typ_weaken_tvar.
+  - asimpl. eapply sub_all; try hauto unfold:ctx_tvar_rename,ctx_tvar_rename_weak ctrs:subtyping use:wf_typ_weaken_tvar.
+    eapply H0.
+    unfold ctx_tvar_rename in *. intros. asimpl. simpl in *.
+    inversion H2; subst; asimpl.
+    + replace (ren_typ (ξ >> S) B1) with (B1 ⟨ξ⟩ ⟨S⟩) by (asimpl; auto).
+      constructor.
+    + replace (ren_typ (ξ >> S) A) with (A ⟨ξ⟩ ⟨S⟩) by (asimpl; auto).
+      constructor; eauto.
+Qed.
